[Progress] Finish Block Allocator

src/Framework/SeparationLogic/Mem.v
@@ -23,6 +23,24 @@ Section GenMem.
       | Some _ => Some v
       end else m a'.
 
+  Definition merge {A AEQ V} (m1: @mem A AEQ V)
+             (m2: @mem A AEQ (V * list V)) : @mem A AEQ (V * list V) :=
+  fun a =>
+    match m1 a with
+    | None => m2 a
+    | Some v =>
+      match m2 a with
+      | None => None
+      | Some vs =>
+        Some (v, fst vs::snd vs)
+      end
+    end.
+
+  Definition addrs_match {A AEQ V1 V2} (m1: @mem A AEQ V1)
+             (m2: @mem A AEQ V2) : Prop :=
+  forall a, m1 a <> None -> m2 a <> None.
+      
+
   Definition delete (m : @mem A AEQ V) (a : A) : @mem A AEQ V :=
     fun a' => if AEQ a' a then None else m a'.
 
