src/Implementations/BatchOperations/Definitions.v
@@ -1,14 +1,10 @@
-Require Import Framework.
-Require DiskLayer CryptoLayer.
-
-Section DiskBatchOperations.
-  Import DiskLayer.
+Require Import Framework CryptoDiskLayer.
 
   Fixpoint write_consecutive a vl :=
   match vl with
   | nil => Ret tt
   | v::vl' =>
-    _ <-| Write a v;
+    _ <- |DO| Write a v;
     _ <- write_consecutive (S a) vl';
     Ret tt
   end.
@@ -17,7 +13,7 @@ Section DiskBatchOperations.
     match count with
     | 0 => Ret nil
     | S count' =>
-      v <-| Read a;
+      v <- |DO| Read _ a;
       vl <- read_consecutive (S a) count';
     Ret (v::vl)
   end.
@@ -25,30 +21,26 @@ Section DiskBatchOperations.
 Fixpoint write_batch al vl :=
   match al, vl with
   | a::al', v::vl' =>
-    _ <-| Write a v;
+    _ <- |DO| Write a v;
     _ <- write_batch al' vl';
     Ret tt            
   | _, _ => Ret tt
   end.
-End DiskBatchOperations.
-
-Section CryptoBatchOperations.
-  Import CryptoLayer.
   
-  Fixpoint encrypt_all k vl :=
-    match vl with
-    | nil => Ret nil
-    | v::vl' =>
-      ev <-| Encrypt k v;
-      evl' <- encrypt_all k vl';
-      Ret (ev::evl')
+Fixpoint encrypt_all k vl :=
+  match vl with
+  | nil => Ret nil
+  | v::vl' =>
+    ev <- |CO| Encrypt k v;
+    evl' <- encrypt_all k vl';
+    Ret (ev::evl')
   end.
 
 Fixpoint decrypt_all k evl :=
   match evl with
   | nil => Ret nil
   | ev::evl' =>
-    v <-| Decrypt k ev;
+    v <- |CO| Decrypt k ev;
     vl' <- decrypt_all k evl';
     Ret (v::vl')
   end.
@@ -57,8 +49,7 @@ Fixpoint hash_all h vl :=
   match vl with
   | nil => Ret h
   | v::vl' =>
-    h' <-| Hash h v;
+    h' <- |CO| Hash h v;
     h'' <- hash_all h' vl';
     Ret h''
   end.
-End CryptoBatchOperations.
