src/Implementations/BlockAllocator/BlockAllocator.v
@@ -1,0 +1,2 @@
+Require Export BlockAllocator.Definitions.
+Require Export BlockAllocator.Facts.
