src/Implementations/BlockAllocator/Specs.v
@@ -1,0 +1,1185 @@
+(*
+Require Import Primitives Layer2 Layer1 Omega.
+Require Import BlockAllocator.
+Require Import L1To2Refinement.Definitions.
+
+Arguments oracle_ok T p o s : simpl never.
+Arguments oracle_refines_to T d1 p o1 o2 : simpl never.
+Arguments rep dh : simpl never.
+
+Theorem alloc_ok:
+  forall o d dh v,
+  << o, d >>
+   (rep dh)
+   (alloc v)
+  << r >>
+   (exists dh',
+    rep dh' *
+     [[(r = None /\ dh' = dh) \/
+       (exists a, r = Some a /\ dh a = None /\ dh' = upd dh a v)%type]])
+   (exists dh',
+    rep dh' *
+     [[(dh' = dh) \/
+       (exists a, dh a = None /\ dh' = upd dh a v)%type]])
+   (exists dh',
+    rep dh' *
+     [[(r = None /\ dh' = dh /\ oracle_refines_to _ d (Alloc v) o (DiskFull::nil)) \/
+       (exists a, r = Some a /\ dh a = None /\ dh' = upd dh a v /\
+             oracle_refines_to _ d (Alloc v) o (BlockNum a::nil))%type]])%pred
+   (exists dh',
+    rep dh' *
+     [[(dh' = dh /\ oracle_refines_to _ d (Alloc v) o (Crash1::nil)) \/
+       (exists a, dh a = None /\ dh' = upd dh a v /\
+             oracle_refines_to _ d (Alloc v) o (CrashAlloc a::nil) )%type]])%pred.
+Proof.
+  unfold alloc, exec; intros.
+  apply remember_oracle_ok; intros.
+  eapply pre_strengthen_aug.
+  2: eapply rep_extract_bitmap.
+  apply extract_exists_aug.
+  intro v0.
+  eapply bind_ok_aug.
+  intros.
+  eapply add_frame.
+  apply read_ok.
+  all: try solve [ simpl; intros; try apply pimpl_refl; cancel].
+  all: try solve [ simpl; intros; try setoid_rewrite rep_merge; cancel].
+
+  intros; destruct_lifts.
+  destruct (lt_dec (get_first_zero (bits (value_to_bits v0_cur))) block_size); simpl in *.
+  {
+    eapply pre_strengthen_aug.
+    2: erewrite rep_extract_block_size_double with (a:= get_first_zero (bits (value_to_bits v0_cur))); eauto.
+    eapply pre_strengthen_aug; [|apply pimpl_exists_l_star_r].
+    apply extract_exists_aug.
+    intro v0.
+    eapply bind_ok_aug.
+    intros; eapply add_frame.
+    apply write_ok.
+
+    all: try solve [ simpl; intros; apply pimpl_refl; cancel].
+    cancel.
+    intros; cancel.
+    rewrite septract_double_split.
+    rewrite sep_star_assoc.
+    setoid_rewrite sep_star_comm at 2.
+    rewrite septract_sep_star_merge.
+    rewrite sep_star_comm, rep_merge; eauto.
+    apply ptsto_complete.
+        
+    simpl; intros; destruct_lifts.
+    intros.
+    eapply bind_ok_aug.
+    intros; eapply add_frame.
+    eapply write_ok.
+    all: try solve [ simpl; intros; try apply pimpl_refl; cancel].
+    intros; simpl; cancel.
+    (* we need folding magic here *)
+    shelve.
+   
+    simpl; intros; destruct_lifts.
+    apply remove_augcons.
+    eapply pre_strengthen.
+    eapply crash_weaken.
+    eapply post_weaken.
+    eapply add_frame.
+    apply ret_ok.
+    all: unfold exec in *.
+    - (* post *)
+      simpl; intros.
+      cancel.
+      right; eexists; intuition eauto.
+      shelve.
+    - cancel.
+      right; eexists; intuition eauto.
+      shelve.
+    - (* Again, folding magic *)
+      shelve.
+      
+    - (* Finished oracle refinement *)
+      simpl; intros; destruct_lifts; cleanup.
+      invert_exec.
+      unfold addr in *; sigT_eq.
+      split_ors; cleanup; try congruence.
+      pred_apply; cancel.
+      
+      right; eexists; intuition eauto.
+      unfold oracle_refines_to; simpl.
+      intuition eauto.
+      destruct (in_dec Layer1.token_dec Layer1.Crash (o1 ++ o0 ++ o2 ++ [Layer1.Cont])).
+      repeat invert_exec; simpl in *.
+      intuition congruence.
+      
+      unfold Disk.read.
+      erewrite ptsto_valid; [| pred_apply; cancel].
+      simpl.
+      destruct (lt_dec (get_first_zero (bits (value_to_bits v0_cur))) block_size); try omega; eauto.
+
+    - simpl; intros; destruct_lifts; cleanup.
+      intuition; cleanup; pred_apply; cancel.
+
+      + left; intuition.
+        unfold oracle_refines_to; simpl.
+        intuition eauto.
+        unfold alloc in *.
+        repeat invert_exec; cleanup.
+        simpl; intuition.
+        repeat invert_exec; cleanup.
+        repeat (try split_ors; invert_exec; simpl in *; cleanup; try congruence).
+        unfold Disk.read, Disk.write, upd_disk in *; cleanup.
+        rewrite upd_eq'; split; intros; eauto.
+        admit. (* solvable by H11 *)
+        congruence.
+        congruence.
+      
+      + right.
+        unfold oracle_refines_to; simpl.
+        repeat invert_exec; cleanup.
+        unfold Disk.read, Disk.write, upd_disk in *; cleanup.
+        simpl; intuition.
+        assume (A : (x = get_first_zero (bits (value_to_bits (fst s))))); cleanup.
+        eexists; intuition eauto.
+        unfold alloc in *.
+        repeat invert_exec; cleanup.
+        repeat (try split_ors; invert_exec; simpl in *; cleanup; try congruence).
+        unfold Disk.read, Disk.write, upd_disk in *; cleanup.
+        rewrite upd_eq'; split; intros; eauto.
+        admit.
+        congruence.
+        congruence.
+        congruence.
+        congruence.
+
+    - simpl; intros; destruct_lifts; cleanup.
+      pred_apply; cancel.
+      rewrite septract_double_split.
+      setoid_rewrite sep_star_comm at 2.
+      rewrite septract_sep_star_merge.
+      eassign dh. admit.
+      apply ptsto_complete.
+      
+      left; intuition.
+      unfold oracle_refines_to; simpl.
+      repeat invert_exec; cleanup.
+      unfold Disk.read, Disk.write, upd_disk in *; cleanup.
+      simpl; intuition.
+      unfold alloc in *.
+      repeat invert_exec; cleanup.
+      repeat (try split_ors; invert_exec; simpl in *; cleanup; try congruence).
+      unfold Disk.read, Disk.write, upd_disk in *; cleanup.
+      rewrite upd_ne; eauto.
+      cleanup.
+      split; intros; eauto.
+      congruence.
+      congruence.
+      congruence.
+
+    - simpl; intros; destruct_lifts; cleanup.
+      pred_apply; cancel.
+      rewrite septract_double_split.
+      rewrite sep_star_assoc.
+      setoid_rewrite sep_star_comm at 2.
+      rewrite septract_sep_star_merge.
+      rewrite sep_star_comm, rep_merge; eauto.
+      apply ptsto_complete.
+      
+      left; intuition.
+      unfold oracle_refines_to; simpl.
+      repeat invert_exec; cleanup.
+      unfold Disk.read, Disk.write, upd_disk in *; cleanup.
+      simpl; intuition.
+      unfold alloc in *.
+      repeat invert_exec; cleanup.
+      repeat (try split_ors; invert_exec; simpl in *; cleanup; try congruence).
+      unfold Disk.read, Disk.write, upd_disk in *; cleanup.
+      split; intros; eauto.
+      congruence.
+      split; intros; eauto.
+      congruence.
+  }
+  {
+    apply remove_augcons.
+    eapply pre_strengthen.
+    eapply crash_weaken.
+    eapply post_weaken.
+    eapply add_frame.
+    apply ret_ok.
+    all: try solve [ simpl; intros; try setoid_rewrite rep_merge; cancel].
+    rewrite sep_star_comm, rep_merge; cancel.
+    all: unfold exec in *.
+    - simpl; intros; destruct_lifts; cleanup.
+      invert_exec; unfold addr in *; sigT_eq.
+      split_ors; cleanup; try congruence.
+      pred_apply; cancel.
+      left; eexists; intuition eauto.
+      unfold oracle_refines_to; simpl.
+      repeat invert_exec; simpl in *.
+      intuition eauto.
+      cleanup.
+      destruct (lt_dec (get_first_zero (bits (value_to_bits v0_cur))) block_size); try omega; eauto.
+
+    - simpl; intros; destruct_lifts; cleanup.
+      intuition; cleanup; pred_apply; cancel.
+
+      + left; intuition.
+        unfold oracle_refines_to; simpl.
+        intuition eauto.
+        unfold alloc in *.
+        repeat invert_exec; cleanup.
+        simpl; intuition.
+        repeat invert_exec; cleanup.
+        repeat (try split_ors; invert_exec; simpl in *; cleanup; try congruence).
+        unfold Disk.read, Disk.write, upd_disk in *; cleanup.
+        split; intros; eauto.
+        congruence.
+      
+      + right.
+        unfold oracle_refines_to; simpl.
+        repeat invert_exec; cleanup.
+        admit.
+  }
+  {
+    unfold exec in *.
+    simpl; intros; destruct_lifts; cleanup.
+    invert_exec.
+    pred_apply; cancel.
+    rewrite sep_star_comm, rep_merge; eauto.
+    
+    left; intuition eauto.
+    unfold oracle_refines_to; simpl.
+    intuition eauto.
+    unfold alloc in *.
+    repeat invert_exec; cleanup.
+    simpl; intuition.
+    repeat invert_exec; cleanup.
+    unfold Disk.read, Disk.write, upd_disk in *; cleanup.
+    erewrite ptsto_valid; [| pred_apply; cancel].
+    split; intros; eauto; congruence.
+    
+    cleanup; repeat invert_exec; simpl in *; cleanup.
+  }
+Admitted.
+
+Theorem read_ok:
+  forall o d a dh,
+  << o, d >>
+   (rep dh)
+   (read a)
+  << r >>
+  (rep dh *
+   [[(r = None /\ (dh a = None \/ a >= block_size)) \/
+     (exists v, r = Some v /\ dh a = Some v)%type]])
+   (rep dh)
+  (rep dh * [[ oracle_refines_to _ d (Layer2.Read a) o (Layer2.Cont::nil) ]] *
+   [[(r = None /\ (dh a = None \/ a >= block_size)) \/
+     (exists v, r = Some v /\ dh a = Some v)%type]])
+   (rep dh * [[ oracle_refines_to _ d (Layer2.Read a) o (Crash1::nil) ]]).
+Proof. Admitted. (*
+  intros.
+  unfold read; simpl.
+
+  unfold rep.
+  repeat (apply hoare_triple_pre_ex; intros).
+  
+  eapply hoare_triple_pimpl;
+    try solve [intros; simpl in *; eauto].
+  eapply hoare_triple_strengthen_pre;
+    [apply read_okay | intros; simpl; cancel].
+
+  simpl. destruct (addr_dec a 1); subst.
+  {
+    intros; simpl.
+    destruct (addr_dec (value_to_nat r) 1); simpl.
+    {
+    eapply hoare_triple_pimpl;
+    try solve [intros; simpl in *; eauto].
+    eapply hoare_triple_strengthen_pre;
+    [apply read_okay | intros; simpl; cancel].
+
+    {
+      intros; simpl.
+      eapply hoare_triple_weaken_post_weak.
+      eapply hoare_triple_weaken_crash_strong.
+      eapply hoare_triple_strengthen_pre.
+      apply ret_okay.
+      
+      intros; simpl in *.
+      destruct_lift H;
+        destruct_lift H0; cleanup;
+          cancel; eauto.
+      
+      intros; simpl in *.
+      destruct_lift H;
+        destruct_lift H0; cleanup;
+          cancel; eauto.
+
+      intros; simpl in *.
+      destruct_lift H;
+        destruct_lift H0;
+        destruct_lift H1;
+        cleanup;
+          cancel; eauto.
+    }
+    intros; simpl in *;
+      destruct_lift H;
+      destruct_lift H0; cleanup;
+        norm; [cancel| intuition (eauto; try omega)].
+    }
+
+    destruct (addr_dec (value_to_nat r) 3); simpl.
+    {
+    eapply hoare_triple_pimpl;
+    try solve [intros; simpl in *; eauto].
+    eapply hoare_triple_strengthen_pre;
+    [apply read_okay | intros; simpl; cancel].
+
+    {
+      intros; simpl.
+      eapply hoare_triple_weaken_post_weak.
+      eapply hoare_triple_weaken_crash_strong.
+      eapply hoare_triple_strengthen_pre.
+      apply ret_okay.
+      
+      intros; simpl in *.
+      destruct_lift H;
+        destruct_lift H0; cleanup;
+          cancel; eauto.
+      
+      intros; simpl in *.
+      destruct_lift H;
+        destruct_lift H0; cleanup;
+          cancel; eauto.
+
+      intros; simpl in *.
+      destruct_lift H;
+        destruct_lift H0;
+        destruct_lift H1;
+        cleanup;
+          cancel; eauto.
+    }
+    intros; simpl in *;
+      destruct_lift H;
+      destruct_lift H0; cleanup;
+        norm; [cancel| intuition (eauto; try omega)].
+    }
+
+      {
+      intros; simpl.
+      eapply hoare_triple_weaken_post_weak.
+      eapply hoare_triple_weaken_crash_strong.
+      eapply hoare_triple_strengthen_pre.
+      apply ret_okay.
+
+      eassign (F * rep dh * ⟦⟦ r = v ⟧⟧).
+      destruct_lift H;
+        cleanup.
+      intros; simpl in *; unfold rep; cancel.
+      
+      unfold rep; intros; simpl in *.
+      destruct_lift H; cleanup.
+      norm; [cancel| intuition (eauto; try omega)].
+      
+
+      intros; simpl in *.
+      unfold rep;
+      destruct_lift H; cleanup;
+      norm; [cancel| intuition (eauto; try omega)].
+      
+      left; split; eauto.
+      left.
+      destruct (addr_dec (value_to_nat v) 0).
+      destruct H8; eauto.
+      destruct (addr_dec (value_to_nat v) 2);
+        destruct H6; eauto.
+      omega.
+    }
+  }
+  
+
+  destruct (addr_dec a 2); subst.
+  {
+    intros; simpl.
+    destruct (addr_dec (value_to_nat r) 2); simpl.
+    {
+    eapply hoare_triple_pimpl;
+    try solve [intros; simpl in *; eauto].
+    eapply hoare_triple_strengthen_pre;
+    [apply read_okay | intros; simpl; cancel].
+
+    {
+      intros; simpl.
+      eapply hoare_triple_weaken_post_weak.
+      eapply hoare_triple_weaken_crash_strong.
+      eapply hoare_triple_strengthen_pre.
+      apply ret_okay.
+      
+      intros; simpl in *.
+      destruct_lift H;
+        destruct_lift H0; cleanup;
+          cancel; eauto.
+      
+      intros; simpl in *.
+      destruct_lift H;
+        destruct_lift H0; cleanup;
+          cancel; eauto.
+
+      intros; simpl in *.
+      destruct_lift H;
+        destruct_lift H0;
+        destruct_lift H1;
+        cleanup;
+          cancel; eauto.
+    }
+    intros; simpl in *;
+      destruct_lift H;
+      destruct_lift H0; cleanup;
+        norm; [cancel| intuition (eauto; try omega)].
+    }
+
+    destruct (addr_dec (value_to_nat r) 3); simpl.
+    {
+    eapply hoare_triple_pimpl;
+    try solve [intros; simpl in *; eauto].
+    eapply hoare_triple_strengthen_pre;
+    [apply read_okay | intros; simpl; cancel].
+
+    {
+      intros; simpl.
+      eapply hoare_triple_weaken_post_weak.
+      eapply hoare_triple_weaken_crash_strong.
+      eapply hoare_triple_strengthen_pre.
+      apply ret_okay.
+      
+      intros; simpl in *.
+      destruct_lift H;
+        destruct_lift H0; cleanup;
+          cancel; eauto.
+      
+      intros; simpl in *.
+      destruct_lift H;
+        destruct_lift H0; cleanup;
+          cancel; eauto.
+
+      intros; simpl in *.
+      destruct_lift H;
+        destruct_lift H0;
+        destruct_lift H1;
+        cleanup;
+          cancel; eauto.
+    }
+    intros; simpl in *;
+      destruct_lift H;
+      destruct_lift H0; cleanup;
+        norm; [cancel| intuition (eauto; try omega)].
+    }
+
+      {
+      intros; simpl.
+      eapply hoare_triple_weaken_post_weak.
+      eapply hoare_triple_weaken_crash_strong.
+      eapply hoare_triple_strengthen_pre.
+      apply ret_okay.
+
+      eassign (F * rep dh * ⟦⟦ r = v ⟧⟧).
+      destruct_lift H;
+        cleanup.
+      intros; simpl in *; unfold rep; cancel.
+      
+      unfold rep; intros; simpl in *.
+      destruct_lift H;
+        cleanup.
+      norm; [cancel| intuition (eauto; try omega)].      
+
+      intros; simpl in *.
+      unfold rep;
+      destruct_lift H;
+        destruct_lift H0;
+        cleanup;
+      norm; [cancel| intuition (eauto; try omega)].
+      
+      left; split; eauto.
+      left.
+      destruct (addr_dec (value_to_nat v) 0).
+      destruct H8; eauto.
+      destruct (addr_dec (value_to_nat v) 1).
+      destruct H7; eauto.
+      omega.
+    }
+  }
+
+  {
+      intros; simpl.
+      eapply hoare_triple_weaken_post_weak.
+      eapply hoare_triple_weaken_crash_strong.
+      eapply hoare_triple_strengthen_pre.
+      apply ret_okay.
+      intros; simpl; rewrite emp_star_r; eauto.
+      destruct_lift H; cancel.
+      destruct_lift H; cancel.
+      left; intuition.      
+      right; omega.
+  }
+
+  intros; simpl.
+  destruct_lift H; cancel.
+Qed.
+
+Lemma exis_lift_absorb:
+  forall A AEQ V T (P: T -> @pred A AEQ V) Q,
+    (exists x, P x) * [[ Q ]] =p=> exists x, (P x * [[Q]]).
+Proof.
+  intros; cancel.
+Qed.
+*)
+
+Theorem write_ok:
+  forall o d dh a v,
+  << o, d >>
+   (rep dh)
+   (write a v)
+  << r >>
+   (exists dh',
+    rep dh' * 
+     [[(r = None /\ dh' = dh /\ dh a = None) \/
+       (r = Some tt /\ dh a <> None /\ dh' = upd dh a v)%type]])
+   (exists dh',
+    rep dh' *
+    [[((dh' = dh) \/
+       (dh a <> None /\ dh' = upd dh a v))%type]])
+   (exists dh',
+    rep dh' * [[ oracle_refines_to _ d (Layer2.Write a v) o (Layer2.Cont::nil) ]] *
+     [[(r = None /\ dh' = dh /\ dh a = None) \/
+       (r = Some tt /\ dh a <> None /\ dh' = upd dh a v)%type]])
+   (exists dh',
+      rep dh' *
+      [[((dh' = dh /\ oracle_refines_to _ d (Layer2.Write a v) o (Crash1::nil)) \/
+       (dh a <> None /\ dh' = upd dh a v /\ oracle_refines_to _ d (Layer2.Write a v) o (Crash2::nil)))%type]]).
+Proof. Admitted. (*
+  intros.
+  unfold write; simpl.
+
+  repeat (apply hoare_triple_pre_ex; intros).
+    eapply hoare_triple_pimpl;
+      try solve [intros; simpl in *; eauto].
+    eapply hoare_triple_strengthen_pre;
+      [apply read_okay | intros; simpl; cancel].
+    
+  intros; simpl; destruct (addr_dec a 1); subst.
+  {
+    intros; simpl.
+    destruct (addr_dec (value_to_nat r) 1); simpl.
+    {
+      eapply hoare_triple_pimpl;
+        try solve [intros; simpl in *; eauto].
+      eapply hoare_triple_strengthen_pre;
+        [apply write_okay | intros; simpl; cancel].
+      
+      {
+        intros; simpl.
+        eapply hoare_triple_weaken_post_weak.
+        eapply hoare_triple_weaken_crash_strong.
+        eapply hoare_triple_strengthen_pre.
+        apply ret_okay.
+        
+        intros; simpl in *.
+        rewrite <- emp_star_r; eauto.
+        
+        intros; unfold rep; simpl in *.
+        norm; [cancel|].
+        eassign (upd dh 1 v).
+        rewrite upd_eq'.
+        repeat rewrite upd_ne; eauto.
+        destruct_lift H;
+          destruct_lift H0;
+          cleanup;
+          intuition (eauto; try omega).
+        rewrite upd_ne; eauto; omega.
+        right; intuition eauto.
+        cleanup.
+
+        intros; unfold rep; simpl in *.
+        norm; [cancel|].
+        eassign (upd dh 1 v).
+        rewrite upd_eq'.
+        repeat rewrite upd_ne; eauto.
+        destruct_lift H;
+          destruct_lift H0;
+          cleanup;
+          intuition (eauto; try omega).
+        rewrite upd_ne; eauto; omega.
+        right; intuition eauto.
+        cleanup.
+      }        
+      intros; unfold rep; simpl in *.
+      destruct_lift H;
+          destruct_lift H0;
+          cleanup;
+        norm; [cancel| intuition (eauto; try omega)].
+    }
+
+    destruct (addr_dec (value_to_nat r) 3); simpl.
+    {
+      eapply hoare_triple_pimpl;
+        try solve [intros; simpl in *; eauto].
+      eapply hoare_triple_strengthen_pre;
+        [apply write_okay | intros; simpl; cancel].
+      {
+        intros; simpl.
+        eapply hoare_triple_weaken_post_weak.
+        eapply hoare_triple_weaken_crash_strong.
+        eapply hoare_triple_strengthen_pre.
+        apply ret_okay.
+        
+        intros; simpl in *.
+        rewrite <- emp_star_r; eauto.
+        
+        intros; unfold rep; simpl in *.
+        norm; [cancel|].
+        eassign (upd dh 1 v).
+        rewrite upd_eq'.
+        repeat rewrite upd_ne; eauto.
+        destruct_lift H;
+          destruct_lift H0;
+          cleanup;
+          intuition (eauto; try omega).
+        rewrite upd_ne; eauto; omega.
+        right; intuition eauto.
+        cleanup.
+
+        intros; unfold rep; simpl in *.
+        norm; [cancel|].
+        eassign (upd dh 1 v).
+        rewrite upd_eq'.
+        repeat rewrite upd_ne; eauto.
+        destruct_lift H;
+          destruct_lift H0;
+          cleanup;
+          intuition (eauto; try omega).
+        rewrite upd_ne; eauto; omega.
+        right; intuition eauto.
+        cleanup.
+      }        
+      intros; unfold rep; simpl in *.
+      destruct_lift H;
+          destruct_lift H0;
+          cleanup;
+        norm; [cancel| intuition (eauto; try omega)].
+    }
+
+      {
+      intros; simpl.
+      eapply hoare_triple_weaken_post_weak.
+      eapply hoare_triple_weaken_crash_strong.
+      eapply hoare_triple_strengthen_pre.
+      apply ret_okay.
+
+      eassign (F * rep dh).
+      destruct_lift H;
+        cleanup.
+      intros; simpl in *; unfold rep; cancel.
+
+      cancel.
+      cancel.
+    }
+  }
+  
+
+  destruct (addr_dec a 2); subst.
+   {
+    intros; simpl.
+    destruct (addr_dec (value_to_nat r) 2); simpl.
+    {
+      eapply hoare_triple_pimpl;
+        try solve [intros; simpl in *; eauto].
+      eapply hoare_triple_strengthen_pre;
+        [apply write_okay | intros; simpl; cancel].
+      destruct_lift H; cleanup.
+      
+      {
+        intros; simpl.
+        eapply hoare_triple_weaken_post_weak.
+        eapply hoare_triple_weaken_crash_strong.
+        eapply hoare_triple_strengthen_pre.
+        apply ret_okay.
+
+        intros; simpl in *.
+        rewrite <- emp_star_r; eauto.
+        
+        intros; unfold rep; simpl in *.
+        norm; [cancel|].
+        eassign (upd dh 2 v).
+        rewrite upd_eq'.
+        repeat rewrite upd_ne; eauto.
+        destruct_lift H;
+          destruct_lift H0;
+          cleanup;
+          intuition (eauto; try omega).
+        rewrite upd_ne; eauto; omega.
+        right; intuition eauto.
+        cleanup.
+
+        intros; unfold rep; simpl in *.
+        norm; [cancel|].
+        eassign (upd dh 2 v).
+        rewrite upd_eq'.
+        repeat rewrite upd_ne; eauto.
+        destruct_lift H;
+          destruct_lift H0;
+          cleanup;
+          intuition (eauto; try omega).
+        rewrite upd_ne; eauto; omega.
+        right; intuition eauto.
+        cleanup.
+      }        
+      intros; unfold rep; simpl in *.
+      destruct_lift H;
+          destruct_lift H0;
+          cleanup;
+        norm; [cancel| intuition (eauto; try omega)].
+    }
+
+    destruct (addr_dec (value_to_nat r) 3); simpl.
+    {
+      eapply hoare_triple_pimpl;
+        try solve [intros; simpl in *; eauto].
+      eapply hoare_triple_strengthen_pre;
+        [apply write_okay | intros; simpl; cancel].
+      {
+        intros; simpl.
+        eapply hoare_triple_weaken_post_weak.
+        eapply hoare_triple_weaken_crash_strong.
+        eapply hoare_triple_strengthen_pre.
+        apply ret_okay.
+        
+        intros; simpl in *.
+        rewrite <- emp_star_r; eauto.
+        
+        intros; unfold rep; simpl in *.
+        norm; [cancel|].
+        eassign (upd dh 2 v).
+        rewrite upd_eq'.
+        repeat rewrite upd_ne; eauto.
+        destruct_lift H;
+          destruct_lift H0;
+          cleanup;
+          intuition (eauto; try omega).
+        rewrite upd_ne; eauto; omega.
+        right; intuition eauto.
+        cleanup.
+
+        intros; unfold rep; simpl in *.
+        norm; [cancel|].
+        eassign (upd dh 2 v).
+        rewrite upd_eq'.
+        repeat rewrite upd_ne; eauto.
+        destruct_lift H;
+          destruct_lift H0;
+          cleanup;
+          intuition (eauto; try omega).
+        rewrite upd_ne; eauto; omega.
+        right; intuition eauto.
+        cleanup.
+      }        
+      intros; unfold rep; simpl in *.
+      destruct_lift H;
+          destruct_lift H0;
+          cleanup;
+        norm; [cancel| intuition (eauto; try omega)].
+    }
+
+      {
+      intros; simpl.
+      eapply hoare_triple_weaken_post_weak.
+      eapply hoare_triple_weaken_crash_strong.
+      eapply hoare_triple_strengthen_pre.
+      apply ret_okay.
+
+      eassign (F * rep dh).
+      destruct_lift H;
+        cleanup.
+      intros; simpl in *; unfold rep; cancel.
+
+      cancel.
+      cancel.
+
+      }
+   }
+
+   {
+      intros; simpl.
+      eapply hoare_triple_weaken_post_weak.
+      eapply hoare_triple_weaken_crash_strong.
+      eapply hoare_triple_strengthen_pre.
+      apply ret_okay.
+
+      eassign (F * rep dh).
+      destruct_lift H;
+        cleanup.
+      intros; simpl in *; unfold rep; cancel.
+      
+      all: cancel.
+   }
+   intros; simpl in *;
+     destruct_lift H; cleanup.
+   cancel; unfold rep; cancel.
+Qed.
+*)
+
+
+
+Theorem free_ok:
+  forall o d dh a,
+  << o, d >>
+   (rep dh)
+   (free a)
+  << r >>
+   (rep (delete dh a))
+   (exists dh',
+       rep dh' *
+       [[ (dh' = dh) \/
+          (dh' = (delete dh a))]])
+   (rep (delete dh a) *
+    [[ oracle_refines_to _ d (Free a) o (Layer2.Cont::nil) ]])
+   (exists dh',
+      rep dh' *
+      [[ (dh' = dh /\ oracle_refines_to _ d (Free a) o (Crash1::nil)) \/
+         (dh' = (delete dh a) /\ oracle_refines_to _ d (Free a) o (Crash2::nil))]]).
+Proof. Admitted. (*
+  intros.
+  unfold free; simpl.
+
+  destruct (addr_dec a 1); subst.
+  {
+    
+
+    intros; simpl.
+    eapply hoare_triple_pimpl;
+      try solve [intros; simpl in *; eauto].
+    eapply hoare_triple_strengthen_pre;
+      [apply unseal_okay | intros; simpl; cancel].
+    apply upd_eq; eauto.
+    simpl; apply can_access_public.
+
+    intros; simpl.
+    destruct (addr_dec (value_to_nat r0) 1); simpl.
+    {
+      eapply hoare_triple_pimpl;
+        try solve [intros; simpl in *; eauto].
+      eapply hoare_triple_strengthen_pre;
+        [apply seal_okay | intros; simpl; cancel].
+    
+      {
+        intros; simpl.
+        eapply hoare_triple_weaken_post_weak.
+        eapply hoare_triple_weaken_crash_strong.
+        eapply hoare_triple_strengthen_pre.
+        apply write_okay.
+        
+        intros; simpl in *.
+        cancel.
+        apply upd_eq'.
+        
+        intros; simpl in *.
+        norm; [cancel|].
+        eassign dh.
+        destruct_lift H;
+          destruct_lift H0;
+          destruct_lift H1;
+          cleanup;
+          intuition (eauto; try omega).
+
+        intros; simpl in *.
+        norm; [cancel|].
+        rewrite delete_eq.
+        repeat rewrite delete_ne; eauto.
+        rewrite nat_to_value_to_nat.
+        destruct_lift H;
+          destruct_lift H0;
+          destruct_lift H1;
+          cleanup;
+          intuition (eauto; try omega).
+        rewrite delete_ne; eauto; omega.
+      }        
+      intros; simpl in *.
+      destruct_lift H;
+          destruct_lift H0;
+          destruct_lift H1;
+          cleanup;
+        norm; [cancel| intuition (eauto; try omega)].
+    }
+
+    destruct (addr_dec (value_to_nat r0) 3); simpl.
+    {
+      eapply hoare_triple_pimpl;
+        try solve [intros; simpl in *; eauto].
+      eapply hoare_triple_strengthen_pre;
+        [apply seal_okay | intros; simpl; cancel].
+    
+      {
+        intros; simpl.
+        eapply hoare_triple_weaken_post_weak.
+        eapply hoare_triple_weaken_crash_strong.
+        eapply hoare_triple_strengthen_pre.
+        apply write_okay.
+        
+        intros; simpl in *.
+        cancel.
+        apply upd_eq'.
+        
+        intros; simpl in *.
+        norm; [cancel|].
+        eassign dh.
+        destruct_lift H;
+          destruct_lift H0;
+          destruct_lift H1;
+          cleanup;
+          intuition (eauto; try omega).
+
+        intros; simpl in *.
+        norm; [cancel|].
+        rewrite delete_eq.
+        repeat rewrite delete_ne; eauto.
+        rewrite nat_to_value_to_nat.
+        destruct_lift H;
+          destruct_lift H0;
+          destruct_lift H1;
+          cleanup;
+          intuition (eauto; try omega).
+        rewrite delete_ne; eauto; omega.
+      }        
+      intros; simpl in *.
+      destruct_lift H;
+          destruct_lift H0;
+          destruct_lift H1;
+          cleanup;
+        norm; [cancel| intuition (eauto; try omega)].
+    }
+
+    {
+      {
+        intros; simpl.
+        eapply hoare_triple_weaken_post_weak.
+        eapply hoare_triple_weaken_crash_strong.
+        eapply hoare_triple_strengthen_pre.
+        apply ret_okay.
+        
+        intros; simpl in *.
+        eassign (((((0 |-> (Public, v, v0) ✶ F) ✶ 1 |-> v1) ✶ 2 |-> v2) ✶ (⟦⟦ r0 = v ⟧⟧))).
+        cancel.
+        
+        intros; simpl in *.
+        norm; [cancel|].
+        eassign dh.
+        destruct_lift H;
+          destruct_lift H0;
+          cleanup;
+          intuition (eauto; try omega).
+
+        intros; simpl in *.
+        norm; [cancel|].
+        rewrite delete_eq.
+        repeat rewrite delete_ne; eauto.
+        destruct_lift H;
+          destruct_lift H0;
+          destruct_lift H1;
+          cleanup;
+          intuition (eauto; try omega).
+        rewrite delete_ne; eauto; omega.
+      }
+    }
+    
+      intros; simpl in *;
+      destruct_lift H;
+          destruct_lift H0;
+          cleanup;
+          norm; [cancel| intuition (eauto; try omega)].
+    intros; simpl in *;
+      destruct_lift H;
+          cleanup;
+        norm; [cancel| intuition (eauto; try omega)].
+  }
+
+  destruct (addr_dec a 2); subst.
+  {
+    unfold rep.
+    repeat (apply hoare_triple_pre_ex; intros).
+    eapply hoare_triple_pimpl;
+      try solve [intros; simpl in *; eauto].
+    eapply hoare_triple_strengthen_pre;
+      [apply read_okay | intros; simpl; cancel].
+
+    intros; simpl.
+    eapply hoare_triple_pimpl;
+      try solve [intros; simpl in *; eauto].
+    eapply hoare_triple_strengthen_pre;
+      [apply unseal_okay | intros; simpl; cancel].
+    apply upd_eq; eauto.
+    simpl; apply can_access_public.
+
+    intros; simpl.
+    destruct (addr_dec (value_to_nat r0) 2); simpl.
+    {
+      eapply hoare_triple_pimpl;
+        try solve [intros; simpl in *; eauto].
+      eapply hoare_triple_strengthen_pre;
+        [apply seal_okay | intros; simpl; cancel].
+    
+      {
+        intros; simpl.
+        eapply hoare_triple_weaken_post_weak.
+        eapply hoare_triple_weaken_crash_strong.
+        eapply hoare_triple_strengthen_pre.
+        apply write_okay.
+        
+        intros; simpl in *.
+        cancel.
+        apply upd_eq'.
+        
+        intros; simpl in *.
+        norm; [cancel|].
+        eassign dh.
+        destruct_lift H;
+          destruct_lift H0;
+          destruct_lift H1;
+          cleanup;
+          intuition (eauto; try omega).
+
+        intros; simpl in *.
+        norm; [cancel|].
+        rewrite delete_eq.
+        repeat rewrite delete_ne; eauto.
+        rewrite nat_to_value_to_nat.
+        destruct_lift H;
+          destruct_lift H0;
+          destruct_lift H1;
+          cleanup;
+          intuition (eauto; try omega).
+        rewrite delete_ne; eauto; omega.
+      }        
+      intros; simpl in *.
+      destruct_lift H;
+          destruct_lift H0;
+          destruct_lift H1;
+          cleanup;
+        norm; [cancel| intuition (eauto; try omega)].
+    }
+
+    destruct (addr_dec (value_to_nat r0) 3); simpl.
+    {
+      eapply hoare_triple_pimpl;
+        try solve [intros; simpl in *; eauto].
+      eapply hoare_triple_strengthen_pre;
+        [apply seal_okay | intros; simpl; cancel].
+    
+      {
+        intros; simpl.
+        eapply hoare_triple_weaken_post_weak.
+        eapply hoare_triple_weaken_crash_strong.
+        eapply hoare_triple_strengthen_pre.
+        apply write_okay.
+        
+        intros; simpl in *.
+        cancel.
+        apply upd_eq'.
+        
+        intros; simpl in *.
+        norm; [cancel|].
+        eassign dh.
+        destruct_lift H;
+          destruct_lift H0;
+          destruct_lift H1;
+          cleanup;
+          intuition (eauto; try omega).
+
+        intros; simpl in *.
+        norm; [cancel|].
+        rewrite delete_eq.
+        repeat rewrite delete_ne; eauto.
+        rewrite nat_to_value_to_nat.
+        destruct_lift H;
+          destruct_lift H0;
+          destruct_lift H1;
+          cleanup;
+          intuition (eauto; try omega).
+        rewrite delete_ne; eauto; omega.
+      }        
+      intros; simpl in *.
+      destruct_lift H;
+          destruct_lift H0;
+          destruct_lift H1;
+          cleanup;
+        norm; [cancel| intuition (eauto; try omega)].
+    }
+
+    {
+      {
+        intros; simpl.
+        eapply hoare_triple_weaken_post_weak.
+        eapply hoare_triple_weaken_crash_strong.
+        eapply hoare_triple_strengthen_pre.
+        apply ret_okay.
+        
+        intros; simpl in *.
+        eassign (((((0 |-> (Public, v, v0) ✶ F) ✶ 1 |-> v1) ✶ 2 |-> v2) ✶ (⟦⟦ r0 = v ⟧⟧))).
+        cancel.
+        
+        intros; simpl in *.
+        norm; [cancel|].
+        eassign dh.
+        destruct_lift H;
+          destruct_lift H0;
+          cleanup;
+          intuition (eauto; try omega).
+
+        intros; simpl in *.
+        norm; [cancel|].
+        rewrite delete_eq.
+        repeat rewrite delete_ne; eauto.
+        destruct_lift H;
+          destruct_lift H0;
+          destruct_lift H1;
+          cleanup;
+          intuition (eauto; try omega).
+        rewrite delete_ne; eauto; omega.
+      }
+    }
+    
+      intros; simpl in *;
+      destruct_lift H;
+          destruct_lift H0;
+          cleanup;
+          norm; [cancel| intuition (eauto; try omega)].
+    intros; simpl in *;
+      destruct_lift H;
+          cleanup;
+        norm; [cancel| intuition (eauto; try omega)].
+  }
+
+
+  {
+    intros; simpl.
+    eapply hoare_triple_weaken_post_weak.
+    eapply hoare_triple_weaken_crash_strong.
+    eapply hoare_triple_strengthen_pre.
+    apply ret_okay.
+
+    all: cancel.
+    cancel.
+    unfold rep.
+    destruct a.
+    unfold delete at 1.
+    destruct (addr_dec 0 0); intuition.
+    repeat rewrite delete_ne; eauto.
+    cancel.
+    rewrite delete_ne; eauto.
+    omega.
+
+    repeat rewrite delete_ne; eauto.
+    cancel.
+    destruct (addr_dec (S a) n1); subst.
+    apply delete_eq.
+    rewrite delete_ne; eauto.
+  }
+Qed.
+ *)
+*)
