src/Implementations/Transaction/Definitions.v
@@ -1,0 +1,46 @@
+Require Import Framework TransactionCacheLayer.
+(*
+Require Import Datatypes PeanoNat.
+Require Import LogParameters.
+ *)
+
+Fixpoint get_latest (txn: list (addr * value)) a :=
+  match txn  with
+  | ad :: txn' =>
+    if addr_eq_dec a (fst ad) then
+      Some (snd ad)
+    else
+      get_latest txn' a
+  | [] =>
+    None
+  end.
+
+Definition start :=
+  _ <- |TCCO| Put [];
+  Ret tt.
+
+Definition write a v :=
+  txn <- |TCCO| Get _;
+  _   <- |TCCO| Put ((a, v)::txn);
+  Ret tt.
+
+Definition commit :=
+  txn <- |TCCO| Get _;
+  let al := fst (split (rev txn)) in
+  let vl := snd (split (rev txn)) in
+  _ <- |TCDO| Write al vl;
+  _ <- |TCCO| Put [];
+  Ret tt.
+
+Definition read a :=
+  txn <- |TCCO| Get _;
+  match get_latest txn a with
+  | Some v =>
+    Ret v
+  | None =>
+    v <- |TCDO| Read a;
+    Ret v
+  end.
+
+Definition transaction_cache_rep txn (s: state TransactionCacheLang) :=
+  fst s = Some txn.
