src/Layers/CachedDisk/CachedDiskLayer.v
@@ -1,0 +1,13 @@
+Require Export CachedDisk.Definitions CachedDisk.Specs.
+
+(*
+Notation "'CacheLayer.oracle'" := CacheLayer.Definitions.oracle.
+Notation "'CacheLayer.prog'" := CacheLayer.Definitions.prog.
+Notation "'CacheLayer.exec'" := CacheLayer.Definitions.exec.
+Notation "'CacheLayer.token_dec'" := CacheLayer.Definitions.token_dec.
+Notation "'CacheLayer.Ret'" := CacheLayer.Definitions.Ret.
+Notation "'CacheLayer.Bind'" := CacheLayer.Definitions.Bind.
+Notation "'CacheLayer.Cont'" := CacheLayer.Definitions.Cont.
+Notation "'CacheLayer.Crash'" := CacheLayer.Definitions.Crash.
+Notation "'CacheLayer.oracle_ok'" := CacheLayer.Definitions.oracle_ok.
+*)
