src/Layers/CachedDisk/Definitions.v
@@ -1,0 +1,14 @@
+Require Import Framework.
+Require Export CryptoDiskLayer CacheLayer.
+Import ListNotations.
+
+Set Implicit Arguments.
+
+Definition CachedDiskOperation :=  HorizontalComposition (CacheOperation addr_dec value) CryptoDiskOperation.
+Definition CachedDiskLang := Build_Language CachedDiskOperation.
+Definition CachedDiskHL := Build_HoareLogic CachedDiskLang.
+
+Notation "'|CDCP|' p" := (@lift_L1 (CacheOperation addr_dec value) CryptoDiskOperation (CacheLang addr_dec value) _ p) (at level 59).
+Notation "'|CDDP|' p" := (@lift_L2 (CacheOperation addr_dec value) CryptoDiskOperation CryptoDiskLang _ p) (at level 59).
+Notation "'|CDCO|' p" := (@lift_L1 (CacheOperation addr_dec value) CryptoDiskOperation (CacheLang addr_dec value) _ (Op (CacheOperation addr_dec value) p)) (at level 59).
+Notation "'|CDDO|' p" := (@lift_L2 (CacheOperation addr_dec value) CryptoDiskOperation CryptoDiskLang _ (Op CryptoDiskOperation p)) (at level 59).
