src/Layers/CryptoDisk/Definitions.v
@@ -1,0 +1,16 @@
+Require Import Framework.
+Require Export DiskLayer CryptoLayer.
+Import ListNotations.
+
+Set Implicit Arguments.
+
+Definition CryptoDiskOperation :=  HorizontalComposition CryptoOperation (DiskOperation addr_dec value).
+Definition CryptoDiskLang := Build_Language CryptoDiskOperation.
+Definition CryptoDiskHL := Build_HoareLogic CryptoDiskLang.
+
+
+Notation "'|CP|' p" := (@lift_L1 CryptoOperation (DiskOperation addr_dec value) CryptoLang _ p) (at level 59).
+Notation "'|DP|' p" := (@lift_L2 CryptoOperation (DiskOperation addr_dec value) (DiskLang addr_dec value) _ p) (at level 59).
+Notation "'|CO|' p" := (@lift_L1 CryptoOperation (DiskOperation addr_dec value) CryptoLang _ (Op CryptoOperation p)) (at level 59).
+Notation "'|DO|' p" := (@lift_L2 CryptoOperation (DiskOperation addr_dec value) (DiskLang addr_dec value) _ (Op (DiskOperation addr_dec value) p)) (at level 59).   
+      
