src/Layers/Disk/Definitions.v
@@ -1,0 +1,176 @@
+Require Import Framework.
+Import ListNotations.
+
+Set Implicit Arguments.
+
+Section DiskLayer.
+
+  Variable A: Type.
+  Variable AEQ: EqDec A.
+  Variable V : Type.
+
+  Inductive token' :=
+  | Crash : token'
+  | Cont : token'.
+
+  Definition token_dec' : forall (t t': token'), {t=t'}+{t<>t'}.
+    decide equality.
+  Defined.
+
+  Definition oracle' := list token'.
+
+  Definition state' :=  @mem A AEQ (V * list V).
+  
+  Inductive prog' : Type -> Type :=
+  | Read : A -> prog' V
+  | Write : A -> V -> prog' unit.
+   
+  Inductive exec' :
+    forall T, oracle' ->  state' -> prog' T -> @Result state' T -> Prop :=
+  | ExecRead : 
+      forall d a vs,
+        d a = Some vs ->
+        exec' [Cont] d (Read a) (Finished d (fst vs))
+             
+  | ExecWrite :
+      forall d a v vs,
+        d a = Some vs ->
+        exec' [Cont] d (Write a v) (Finished (upd d a (v, (fst vs::snd vs))) tt)
+ 
+  | ExecCrash :
+      forall T d (p: prog' T),
+        exec' [Crash] d p (Crashed d).
+
+  Hint Constructors exec' : core.
+
+  Definition weakest_precondition' T (p: prog' T) :=
+   match p in prog' T' return (T' -> state' -> Prop) -> oracle' -> state' -> Prop with
+   | Read a =>
+     (fun Q o s =>
+       exists vs,
+         o = [Cont] /\
+         s a = Some vs /\
+         Q (fst vs) s)
+   | Write a v =>
+     (fun Q o s =>
+       exists vs,
+       o = [Cont] /\
+       s a = Some vs /\
+       Q tt (upd s a (v, (fst vs::snd vs))))
+   end.
+
+  Definition weakest_crash_precondition' T (p: prog' T) :=
+    fun (Q: state' -> Prop) o (s: state') => o = [Crash] /\ Q s.
+
+  Definition strongest_postcondition' T (p: prog' T) :=
+   match p in prog' T' return (oracle' -> state' -> Prop) -> T' -> state' -> Prop with
+   | Read a =>
+     fun P t s' =>
+       exists s vs,
+         P [Cont] s /\
+         s' = s /\
+         s a = Some vs /\
+         t = fst vs
+   | Write a v =>
+     fun P t s' =>
+       exists s vs,
+         P [Cont] s /\
+         s' = upd s a (v, (fst vs::snd vs)) /\
+         s a = Some vs /\
+         t = tt
+   end.
+
+  Definition strongest_crash_postcondition' T (p: prog' T) :=
+    fun (P: oracle' -> state' -> Prop) s' => P [Crash] s'.
+
+
+  Theorem sp_complete':
+    forall T (p: prog' T) P (Q: _ -> _ -> Prop),
+      (forall t s', strongest_postcondition' p P t s' -> Q t s') <->
+      (forall o s s' t, P o s -> exec' o s p (Finished s' t) -> Q t s').
+  Proof.
+    intros; destruct p; simpl; eauto;
+    split; intros;
+    try inversion H1; cleanup;
+    eapply H; eauto;
+    eexists; eauto.
+  Qed.
+
+  Theorem scp_complete':
+    forall T (p: prog' T) P (Q:  _ -> Prop),
+      (forall s', strongest_crash_postcondition' p P s' -> Q s') <->
+      (forall o s s', P o s -> exec' o s p (Crashed s') -> Q s').
+  Proof.
+    intros; destruct p; simpl; eauto;
+    split; intros;
+    try inversion H1; cleanup;
+    eapply H; eauto.
+  Qed.
+
+
+  Theorem wp_complete':
+    forall T (p: prog' T) H Q,
+      (forall o s, H o s -> weakest_precondition' p Q o s) <->
+      (forall o s, H o s -> (exists s' v, exec' o s p (Finished s' v) /\ Q v s')).
+  Proof.
+    intros; destruct p; simpl; eauto;
+    split; intros;
+    try specialize H0 with (1:= X);
+    cleanup; eauto;
+    try inversion H0; cleanup; eauto.
+    do 2 eexists; intuition eauto.
+    constructor; eauto.
+  Qed.
+  
+  Theorem wcp_complete':
+    forall T (p: prog' T) H C,
+      (forall o s, H o s -> weakest_crash_precondition' p C o s) <->
+      (forall o s, H o s -> (exists s', exec' o s p (Crashed s') /\ C s')).
+  Proof.
+    unfold weakest_crash_precondition';
+    intros; destruct p; simpl; eauto;
+    split; intros;
+    specialize H0 with (1:= X);
+    cleanup; eauto;
+    inversion H0; cleanup; eauto.
+  Qed.
+
+  Theorem exec_deterministic_wrt_oracle' :
+    forall o s T (p: prog' T) ret1 ret2,
+      exec' o s p ret1 ->
+      exec' o s p ret2 ->
+      ret1 = ret2.
+  Proof.
+    intros; destruct p; simpl in *; cleanup;
+    repeat
+      match goal with
+      | [H: exec' _ _ _ _ |- _] =>
+        inversion H; clear H; cleanup
+      end; eauto.
+  Qed.
+  
+  Definition DiskOperation :=
+    Build_Operation
+      (list_eq_dec token_dec')
+      prog'
+      exec'
+      weakest_precondition'
+      weakest_crash_precondition'
+      strongest_postcondition'
+      strongest_crash_postcondition'
+      wp_complete'
+      wcp_complete'
+      sp_complete'
+      scp_complete'
+      exec_deterministic_wrt_oracle'.
+  
+  Definition DiskLang := Build_Language DiskOperation.
+  Definition DiskHL := Build_HoareLogic DiskLang.
+
+Notation "| p |" := (Op DiskOperation p)(at level 60).
+Notation "x <-| p1 ; p2" := (Bind (Op DiskOperation p1) (fun x => p2))(right associativity, at level 60). 
+Notation "p >> s" := (p s) (right associativity, at level 60, only parsing).
+
+End DiskLayer.
+
+Arguments Read {_}.
