src/Layers/LoggedDisk/LoggedDiskLayer.v
@@ -1,0 +1,1 @@
+Require Export Layers.LoggedDisk.Definitions.
