src/Layers/LoggedDiskLayer/LoggedDiskLayer.v
@@ -1,3 +1,0 @@
-Require Export LoggedDiskLayer.Definitions.
-
-Notation "'LoggedDisk.Read'" := LoggedDiskLayer.Definitions.Read.
