src/Layers/TransactionCache/Definitions.v
@@ -1,0 +1,14 @@
+Require Import Framework.
+Require Export LoggedDiskLayer StorageLayer.
+Import ListNotations.
+
+Set Implicit Arguments.
+
+Definition TransactionCacheOperation :=  HorizontalComposition (StorageOperation (list (addr * value))) LoggedDiskOperation.
+Definition TransactionCacheLang := Build_Language TransactionCacheOperation.
+Definition TransactionCacheHL := Build_HoareLogic TransactionCacheLang.
+
+Notation "'|TCCP|' p" := (@lift_L1 (StorageOperation (list (addr * value))) LoggedDiskOperation (StorageLang (list (addr * value))) _ p) (at level 59).
+Notation "'|TCDP|' p" := (@lift_L2 (StorageOperation (list (addr * value))) LoggedDiskOperation LoggedDiskLang _ p) (at level 59).
+Notation "'|TCCO|' p" := (@lift_L1 (StorageOperation (list (addr * value))) LoggedDiskOperation (StorageLang (list (addr * value))) _ (Op (StorageOperation (list (addr * value))) p)) (at level 59).
+Notation "'|TCDO|' p" := (@lift_L2 (StorageOperation (list (addr * value))) LoggedDiskOperation LoggedDiskLang _ (Op LoggedDiskOperation p)) (at level 59).
